Improve performance of lemma FirePEConfluence

isa.dfy
@@ -1,7 +1,7 @@
 type ChannelIndex = int
 type PEIndex = int
-
 type Value = int
+type Channel = seq<Value>
 
 datatype CarryState = CarryI | CarryB1 | CarryB2
 datatype SteerState = SteerI | SteerA | SteerB
@@ -95,31 +95,10 @@ datatype ProcessingElement =
     }
 }
 
-type Channel = seq<Value>
-
-// datatype Channel = Channel(buffer: seq<Value>)
-// {
-//     function method Length(): int
-//     {
-//         |buffer|
-//     }
-
-//     function method Send(value: Value): (newChannel: Channel)
-//     {
-//         Channel(buffer + [value])
-//     }
-
-//     function method Receive(): (Value, Channel)
-//         requires |buffer| > 0
-//     {
-//         (buffer[0], Channel(buffer[1..]))
-//     }
-// }
-
 datatype DataflowProgramState = DataflowProgramState(channels: seq<Channel>, processingElements: seq<ProcessingElement>)
 {
     // Returns if the dataflow program is well-formed
-    predicate Wellformed()
+    predicate {:opaque} WellFormed()
     {
         // Inputs & outputs are valid channel indices
         // Inputs do not overlap
@@ -131,15 +110,14 @@ datatype DataflowProgramState = DataflowProgramState(channels: seq<Channel>, pro
             forall idx :: idx in pe.Inputs() || idx in pe.Outputs() ==>
             0 <= idx < |channels|;
 
-        var noIOOverlap := 
-            forall pe1 :: pe1 in processingElements ==>
-            forall pe2 :: pe2 in processingElements && pe1 != pe2 ==>
-                (forall i :: i in pe1.Inputs() ==> i !in pe2.Inputs()) &&
-                (forall i :: i in pe1.Outputs() ==> i !in pe2.Outputs());
-
-        var distinctPEs :=
+        var noIOOverlap :=
             forall i, j :: 0 <= i < j < |processingElements| ==>
-            processingElements[i] != processingElements[j];
+                (forall k :: k in processingElements[i].Inputs() ==> k !in processingElements[j].Inputs()) &&
+                (forall k :: k in processingElements[i].Outputs() ==> k !in processingElements[j].Outputs());
+
+        // var distinctPEs :=
+        //     forall i, j :: 0 <= i < j < |processingElements| ==>
+        //     processingElements[i] != processingElements[j];
 
         var distinctInputChannels :=
             forall pe :: pe in processingElements ==>
@@ -151,30 +129,70 @@ datatype DataflowProgramState = DataflowProgramState(channels: seq<Channel>, pro
             forall i, j :: 0 <= i < j < |pe.Outputs()| ==>
             pe.Outputs()[i] != pe.Outputs()[j];
 
-        validChannelIndices && noIOOverlap && distinctPEs && distinctInputChannels && distinctOutputChannels
+        validChannelIndices && noIOOverlap && distinctInputChannels && distinctOutputChannels
     }
 
     // Returns if the given PE is fireable in the dataflow program
     predicate IsFireable(idx: PEIndex)
-        requires Wellformed()
+        requires WellFormed()
         requires 0 <= idx < |processingElements|
     {
-        forall ChannelIndex :: ChannelIndex in processingElements[idx].WaitingInputs() ==>
-            ChannelIndex in processingElements[idx].Inputs() && // TODO: this is not necessary
-            |channels[ChannelIndex]| != 0
+        reveal_WellFormed();
+        forall i :: i in processingElements[idx].WaitingInputs() ==> |channels[i]| != 0
     }
 
-    function Multicast(value: Value, outputs: seq<ChannelIndex>): DataflowProgramState
-        requires Wellformed()
+    function UpdatePE(idx: PEIndex, pe: ProcessingElement): (result: DataflowProgramState)
+        requires WellFormed()
+        requires 0 <= idx < |processingElements|
+        requires pe.Inputs() == processingElements[idx].Inputs()
+        requires pe.Outputs() == processingElements[idx].Outputs()
+        ensures result.WellFormed()
+    {
+        reveal_WellFormed();
+        DataflowProgramState(channels, processingElements[idx := pe])
+    }
+
+    function Receive(channelIdx: ChannelIndex): (Value, DataflowProgramState)
+        requires WellFormed()
+        requires 0 <= channelIdx < |channels|
+        requires |channels[channelIdx]| > 0
+
+        ensures Receive(channelIdx).1.WellFormed()
+        // ensures var result := Receive(channelIdx).1;
+        //         result.WellFormed() &&
+        //         |result.channels| == |channels| &&
+        //         forall i :: 0 <= i < |channels| ==>
+        //             (i == channelIdx ==> result.channels[i] == channels[i][1..]) &&
+        //             (i != channelIdx ==> result.channels[i] == channels[i])
+    {
+        reveal_WellFormed();
+        (channels[channelIdx][0], DataflowProgramState(channels[channelIdx := channels[channelIdx][1..]], processingElements))
+    }
+
+    function Send(value: Value, channelIdx: ChannelIndex): (result: DataflowProgramState)
+        requires WellFormed()
+        requires 0 <= channelIdx < |channels|
+        ensures result.WellFormed()
+        // ensures |result.channels| == |channels| &&
+        //         forall i :: 0 <= i < |channels| ==>
+        //             (i == channelIdx ==> result.channels[i] == channels[i] + [value]) &&
+        //             (i != channelIdx ==> result.channels[i] == channels[i])
+    {
+        reveal_WellFormed();
+        DataflowProgramState(channels[channelIdx := channels[channelIdx] + [value]], processingElements)
+    }
+
+    function Multicast(value: Value, outputs: seq<ChannelIndex>): (result: DataflowProgramState)
+        requires WellFormed()
         requires forall idx :: idx in outputs ==> 0 <= idx < |channels|
         requires forall i, j :: 0 <= i < j < |outputs| ==> outputs[i] != outputs[j]
 
-        ensures var result := Multicast(value, outputs);
-                |result.channels| == |channels| &&
+        ensures |result.channels| == |channels| &&
                 result.processingElements == processingElements &&
                 forall idx :: 0 <= idx < |channels| ==>
                     (idx !in outputs ==> result.channels[idx] == channels[idx]) &&
                     (idx in outputs ==> result.channels[idx] == channels[idx] + [value])
+        ensures result.WellFormed()
 
         decreases outputs
     {
@@ -183,19 +201,18 @@ datatype DataflowProgramState = DataflowProgramState(channels: seq<Channel>, pro
         else
             var idx := outputs[0];
             assert idx in outputs;
-            var newChannels := channels[idx := channels[idx] + [value]];
-            var newState := DataflowProgramState(newChannels, processingElements);
+            var newState := this.Send(value, idx);
             assert forall idx :: idx in outputs[1..] ==> idx in outputs;
+            reveal_WellFormed();
             newState.Multicast(value, outputs[1..])
     }
 
     // Fires the specified PE and transition to a new state
     function {:opaque} FirePE(idx: PEIndex): (result: DataflowProgramState)
         requires 0 <= idx < |processingElements|
-        requires Wellformed()
+        requires WellFormed()
         requires IsFireable(idx)
 
-        ensures Wellformed()
         ensures |result.channels| == |channels|
         ensures |result.processingElements| == |processingElements|
 
@@ -205,78 +222,52 @@ datatype DataflowProgramState = DataflowProgramState(channels: seq<Channel>, pro
         ensures forall i :: 0 <= i < |result.processingElements| && i != idx
                             ==> result.processingElements[i] == processingElements[i]
 
-        // Characterize how the channels change after firing
-        ensures forall i :: i in processingElements[idx].WaitingInputs() && i in processingElements[idx].WaitingOutputs() ==>
-                            |result.channels[i]| >= 1 && result.channels[i][..|result.channels[i]| - 1] == channels[i][1..]
-
-        ensures forall i :: i in processingElements[idx].WaitingInputs() && i !in processingElements[idx].WaitingOutputs() ==>
-                            result.channels[i] == channels[i][1..]
-
-        ensures forall i :: i !in processingElements[idx].WaitingInputs() && i in processingElements[idx].WaitingOutputs() ==>
-                            |result.channels[i]| >= 1 && result.channels[i][..|result.channels[i]| - 1] == channels[i]
-
-        ensures forall i :: i !in processingElements[idx].WaitingInputs() && i !in processingElements[idx].WaitingOutputs() && 0 <= i < |result.channels| ==>
-                            result.channels[i] == channels[i]
+        ensures result.WellFormed()
     {
+        reveal_WellFormed();
         var pe := processingElements[idx];
         match pe
             case AddOperator(a, b, outputs) =>
-                assert a in pe.Inputs() && b in pe.Inputs();
-                assert outputs <= pe.Outputs();
-                // assert a == pe.Inputs()[0] && b == pe.Inputs()[1];
-                // assert a != b;
+                assert a in pe.WaitingInputs() && b in pe.WaitingInputs();
+                assert outputs == pe.Outputs();
+                assert a == pe.Inputs()[0] && b == pe.Inputs()[1];
 
-                var valA := channels[a][0];
-                var valB := channels[b][0];
-                var newChannels := channels[a := channels[a][1..]][b := channels[b][1..]];
-                var newState := DataflowProgramState(newChannels, processingElements);
-
+                var (valA, newState) := this.Receive(a);
+                var (valB, newState) := newState.Receive(b);
                 newState.Multicast(valA + valB, outputs)
 
             case SteerOperator(steer, state, d, a, outputs) =>
                 match state {
                     case SteerI =>
-                        assert d in pe.Inputs();
+                        assert d in pe.WaitingInputs();
 
-                        var valD := channels[d][0];
-                        var newChannels := channels[d := channels[d][1..]];
+                        var (valD, newState) := this.Receive(d);
                         var updatedPE := if (valD == 0 && !steer) || (valD != 0 && steer)
-                                            then SteerOperator(steer, SteerA, d, a, outputs)
-                                            else SteerOperator(steer, SteerB, d, a, outputs);
-                        var newPEs := processingElements[idx := updatedPE];
-                        
-                        DataflowProgramState(newChannels, newPEs)
+                                         then SteerOperator(steer, SteerA, d, a, outputs)
+                                         else SteerOperator(steer, SteerB, d, a, outputs);
+                        newState.UpdatePE(idx, updatedPE)
 
                     case SteerA =>
                         assert a in pe.Inputs();
-                        var valA := channels[a][0];
-                        var newChannels := channels[a := channels[a][1..]];
-                        var newPEs := processingElements[idx := SteerOperator(steer, SteerI, d, a, outputs)];
-                        var newState := DataflowProgramState(newChannels, newPEs);
-                        
-                        assert forall i :: 0 <= i < |newPEs| ==> newPEs[i].Inputs() == processingElements[i].Inputs();
-                        assert processingElements[idx].Outputs() == outputs;
 
+                        var (valA, newState) := this.Receive(a);
+                        var newState := newState.UpdatePE(idx, SteerOperator(steer, SteerI, d, a, outputs));
                         newState.Multicast(valA , outputs)
 
                     case SteerB =>
                         assert a in pe.Inputs();
-                        var newChannels := channels[a := channels[a][1..]];
-                        var newPEs := processingElements[idx := SteerOperator(steer, SteerI, d, a, outputs)];
-                        var newState := DataflowProgramState(newChannels, newPEs);
-                        newState
-
+                        var (_, newState) := this.Receive(a);
+                        newState.UpdatePE(idx, SteerOperator(steer, SteerI, d, a, outputs))
                 }
 
             case SelectOperator(d, a, b, outputs) =>
-                assert d in pe.Inputs() && a in pe.Inputs() && b in pe.Inputs();
-                assert outputs <= pe.Outputs();
-
-                var valD := channels[d][0];
-                var valA := channels[a][0];
-                var valB := channels[b][0];
-                var newChannels := channels[d := channels[d][1..]][a := channels[a][1..]][b := channels[b][1..]];
-                var newState := DataflowProgramState(newChannels, processingElements);
+                assert d in pe.WaitingInputs() && a in pe.WaitingInputs() && b in pe.WaitingInputs();
+                assert outputs == pe.Outputs();
+                assert d == pe.Inputs()[0] && a == pe.Inputs()[1] && b == pe.Inputs()[2];
+                
+                var (valD, newState) := this.Receive(d);
+                var (valA, newState) := newState.Receive(a);
+                var (valB, newState) := newState.Receive(b);
 
                 if valD == 1 then
                     newState.Multicast(valA, outputs)
@@ -286,124 +277,201 @@ datatype DataflowProgramState = DataflowProgramState(channels: seq<Channel>, pro
             case CarryOperator(state, d, a, b, outputs) =>
                 match state {
                     case CarryI =>
-                        assert a in pe.Inputs();
+                        assert a in pe.WaitingInputs();
 
-                        var valA := channels[a][0];
-                        var newChannels := channels[a := channels[a][1..]];
-                        var newPEs := processingElements[idx := CarryOperator(CarryB1, d, a, b, outputs)];
-                        var newState := DataflowProgramState(newChannels, newPEs);
-
-                        assert forall i :: 0 <= i < |newPEs| ==> newPEs[i].Inputs() == processingElements[i].Inputs();
-                        assert processingElements[idx].Outputs() == outputs;
-
+                        var (valA, newState) := this.Receive(a);
+                        var newState := newState.UpdatePE(idx, CarryOperator(CarryB1, d, a, b, outputs));
                         newState.Multicast(valA, outputs)
 
                     case CarryB1 =>
-                        assert d in pe.Inputs();
+                        assert d in pe.WaitingInputs();
 
-                        var valD := channels[d][0];
-                        var newChannels := channels[d := channels[d][1..]];
-
+                        var (valD, newState) := this.Receive(d);
                         var updatedPE := if valD == 0 then CarryOperator(CarryI, d, a, b, outputs)
                                                       else CarryOperator(CarryB2, d, a, b, outputs);
-                        var newPEs := processingElements[idx := updatedPE];
-
-                        DataflowProgramState(newChannels, newPEs)
+                        newState.UpdatePE(idx, updatedPE)
                         
                     case CarryB2 =>
-                        assert b in pe.Inputs();
+                        assert b in pe.WaitingInputs();
 
-                        var valB := channels[b][0];
-                        var newChannels := channels[b := channels[b][1..]];
-                        var newPEs := processingElements[idx := CarryOperator(CarryB1, d, a, b, outputs)];
-                        var newState := DataflowProgramState(newChannels, newPEs);
-
-                        assert forall i :: 0 <= i < |newPEs| ==> newPEs[i].Inputs() == processingElements[i].Inputs();
-                        assert processingElements[idx].Outputs() == outputs;
-
+                        var (valB, newState) := this.Receive(b);
+                        var newState := newState.UpdatePE(idx, CarryOperator(CarryB1, d, a, b, outputs));
                         newState.Multicast(valB, outputs)
                 }
 
             case OrderOperator(a, b, outputs) =>
-                assert a in pe.Inputs() && b in pe.Inputs();
+                assert a in pe.WaitingInputs() && b in pe.WaitingInputs();
                 assert outputs <= pe.Outputs();
+                assert a == pe.Inputs()[0] && b == pe.Inputs()[1];
                 
-                var valA := channels[a][0];
-                var valB := channels[b][0];
-                var newChannels := channels[a := channels[a][1..]][b := channels[b][1..]];
-                var newState := DataflowProgramState(newChannels, processingElements);
-
+                var (valA, newState) := this.Receive(a);
+                var (valB, newState) := newState.Receive(b);
                 newState.Multicast(valB, outputs)
 
             case MergeOperator(state, d, a, b, outputs) =>
                 match state {
                     case MergeI =>
-                        assert d in pe.Inputs();
+                        assert d in pe.WaitingInputs();
 
-                        var valD := channels[d][0];
-                        var newChannels := channels[d := channels[d][1..]];
-
+                        var (valD, newState) := this.Receive(d);
                         var updatedPE := if valD == 0 then MergeOperator(MergeA, d, a, b, outputs)
                                                       else MergeOperator(MergeB, d, a, b, outputs);
-                        var newPEs := processingElements[idx := updatedPE];
-
-                        DataflowProgramState(newChannels, newPEs)
+                        newState.UpdatePE(idx, updatedPE)
 
                     case MergeA =>
-                        assert a in pe.Inputs();
+                        assert a in pe.WaitingInputs();
 
-                        var valA := channels[a][0];
-                        var newChannels := channels[a := channels[a][1..]];
-                        var newPEs := processingElements[idx := MergeOperator(MergeI, d, a, b, outputs)];
-                        var newState := DataflowProgramState(newChannels, newPEs);
-
-                        assert forall i :: 0 <= i < |newPEs| ==> newPEs[i].Inputs() == processingElements[i].Inputs();
-                        assert processingElements[idx].Outputs() == outputs;
-
+                        var (valA, newState) := this.Receive(a);
+                        var newState := newState.UpdatePE(idx, MergeOperator(MergeI, d, a, b, outputs));
                         newState.Multicast(valA, outputs)
 
                     case MergeB =>
-                        assert b in pe.Inputs();
-                        assert outputs <= pe.Outputs();
+                        assert b in pe.WaitingInputs();
 
-                        var valB := channels[b][0];
-                        var newChannels := channels[b := channels[b][1..]];
-                        var newPEs := processingElements[idx := MergeOperator(MergeI, d, a, b, outputs)];
-                        var newState := DataflowProgramState(newChannels, newPEs);
-
-                        assert forall i :: 0 <= i < |newPEs| ==> newPEs[i].Inputs() == processingElements[i].Inputs();
+                        var (valB, newState) := this.Receive(b);
+                        var newState := newState.UpdatePE(idx, MergeOperator(MergeI, d, a, b, outputs));
                         newState.Multicast(valB, outputs)
                 }
     }
 
-    predicate AreBothFireable(idx1: PEIndex, idx2: PEIndex)
-        requires Wellformed()
+    // Specifies how a particular channel changes after Fire(idx)
+    lemma FirePEChannelChange(idx: PEIndex, channelIdx: ChannelIndex)
+        requires 0 <= idx < |processingElements|
+        requires 0 <= channelIdx < |channels|
+        requires WellFormed()
+        requires IsFireable(idx)
+
+        ensures |FirePE(idx).channels| == |channels|
+        ensures |FirePE(idx).processingElements| == |processingElements|
+
+        ensures FirePE(idx).processingElements[idx].Inputs() == processingElements[idx].Inputs()
+        ensures FirePE(idx).processingElements[idx].Outputs() == processingElements[idx].Outputs()
+
+        ensures forall i :: 0 <= i < |FirePE(idx).processingElements| && i != idx
+                            ==> FirePE(idx).processingElements[i] == processingElements[i]
+
+        requires WellFormed()
+
+        ensures var original := channels[channelIdx];
+                var result := FirePE(idx).channels[channelIdx];
+                var pe := processingElements[idx];
+                
+                (channelIdx in pe.WaitingInputs() && channelIdx in pe.WaitingOutputs() ==>
+                 |result| >= 1 && result[..|result| - 1] == original[1..]) &&
+
+                (channelIdx in pe.WaitingInputs() && channelIdx !in pe.WaitingOutputs() ==>
+                 result == original[1..]) &&
+
+                (channelIdx !in pe.WaitingInputs() && channelIdx in pe.WaitingOutputs() ==>
+                 |result| >= 1 && result[..|result| - 1] == original) &&
+
+                (channelIdx !in pe.WaitingInputs() && channelIdx !in pe.WaitingOutputs() ==>
+                 result == original)
     {
-        0 <= idx1 < |processingElements| &&
-        0 <= idx2 < |processingElements| &&
-        IsFireable(idx1) && IsFireable(idx2)
+        reveal_FirePE();
+
+        var pe := processingElements[idx];
+        match pe
+            case AddOperator(a, b, outputs) => {
+                assert a in pe.WaitingInputs() && b in pe.WaitingInputs();
+                assert outputs == pe.Outputs();
+                assert a == pe.Inputs()[0] && b == pe.Inputs()[1];
+            }
+
+            case SelectOperator(d, a, b, outputs) => {
+                assert outputs == pe.Outputs();
+                assert d == pe.Inputs()[0] && a == pe.Inputs()[1] && b == pe.Inputs()[2];
+            }
+
+            case OrderOperator(a, b, outputs) => {
+                assert outputs <= pe.Outputs();
+                assert a == pe.Inputs()[0] && b == pe.Inputs()[1];
+            }
+
+            case _ => {}
+    }
+
+    lemma FirePEChannelChangeAuto(idx: PEIndex)
+        requires 0 <= idx < |processingElements|
+        requires WellFormed()
+        requires IsFireable(idx)
+
+        ensures |FirePE(idx).channels| == |channels|
+        ensures |FirePE(idx).processingElements| == |processingElements|
+
+        ensures FirePE(idx).processingElements[idx].Inputs() == processingElements[idx].Inputs()
+        ensures FirePE(idx).processingElements[idx].Outputs() == processingElements[idx].Outputs()
+
+        ensures forall i :: 0 <= i < |FirePE(idx).processingElements| && i != idx
+                            ==> FirePE(idx).processingElements[i] == processingElements[i]
+
+        requires WellFormed()
+
+        ensures forall channelIdx :: 0 <= channelIdx < |channels| ==> (
+                    var original := channels[channelIdx];
+                    var result := FirePE(idx).channels[channelIdx];
+                    var pe := processingElements[idx];
+                    
+                    (channelIdx in pe.WaitingInputs() && channelIdx in pe.WaitingOutputs() ==>
+                     |result| >= 1 && result[..|result| - 1] == original[1..]) &&
+
+                    (channelIdx in pe.WaitingInputs() && channelIdx !in pe.WaitingOutputs() ==>
+                     result == original[1..]) &&
+
+                    (channelIdx !in pe.WaitingInputs() && channelIdx in pe.WaitingOutputs() ==>
+                     |result| >= 1 && result[..|result| - 1] == original) &&
+
+                    (channelIdx !in pe.WaitingInputs() && channelIdx !in pe.WaitingOutputs() ==>
+                     result == original)
+                )
+    {
+        forall channelIdx | 0 <= channelIdx < |channels|
+            ensures (
+                var original := channels[channelIdx];
+                var result := FirePE(idx).channels[channelIdx];
+                var pe := processingElements[idx];
+                
+                (channelIdx in pe.WaitingInputs() && channelIdx in pe.WaitingOutputs() ==>
+                    |result| >= 1 && result[..|result| - 1] == original[1..]) &&
+
+                (channelIdx in pe.WaitingInputs() && channelIdx !in pe.WaitingOutputs() ==>
+                    result == original[1..]) &&
+
+                (channelIdx !in pe.WaitingInputs() && channelIdx in pe.WaitingOutputs() ==>
+                    |result| >= 1 && result[..|result| - 1] == original) &&
+
+                (channelIdx !in pe.WaitingInputs() && channelIdx !in pe.WaitingOutputs() ==>
+                    result == original)
+            )
+        {
+            var original := channels[channelIdx];
+            var result := FirePE(idx).channels[channelIdx];
+            var pe := processingElements[idx];
+            FirePEChannelChange(idx, channelIdx);
+        }
     }
 
     lemma CommutableFiring(idx1: PEIndex, idx2: PEIndex)
-        requires Wellformed()
+        requires WellFormed()
         requires idx1 != idx2
         requires 0 <= idx1 < |processingElements|
         requires 0 <= idx2 < |processingElements|
         requires IsFireable(idx1)
         requires IsFireable(idx2)
-        ensures FirePE(idx1).Wellformed()
+        ensures FirePE(idx1).WellFormed()
         ensures FirePE(idx1).IsFireable(idx2)
     {
         reveal_FirePE();
     }
 
     // Output values do not depend on the channels other than WaitingInputs()
-    lemma FirePEDependency(state1: DataflowProgramState, state2: DataflowProgramState, idx: PEIndex)
-        requires state1.Wellformed() && state2.Wellformed()
+    lemma FirePEDependency(state1: DataflowProgramState, state2: DataflowProgramState, idx: PEIndex, outputIdx: ChannelIndex)
+        requires state1.WellFormed() && state2.WellFormed()
         requires |state1.channels| == |state2.channels|
         requires 0 <= idx < |state1.processingElements| == |state2.processingElements|
         requires state1.processingElements[idx] == state2.processingElements[idx]
         requires state1.IsFireable(idx) && state2.IsFireable(idx)
+        requires outputIdx in state1.processingElements[idx].WaitingOutputs()
 
         // Same input values
         requires forall i :: i in state1.processingElements[idx].WaitingInputs() ==>
@@ -413,23 +481,48 @@ datatype DataflowProgramState = DataflowProgramState(channels: seq<Channel>, pro
         ensures var pe := state1.processingElements[idx];
                 var result1 := state1.FirePE(idx);
                 var result2 := state2.FirePE(idx);
-                forall i :: i in pe.WaitingOutputs() ==>
-                result1.channels[i][|result1.channels[i]| - 1] == result2.channels[i][|result2.channels[i]| - 1] &&
+                result1.WellFormed() &&
+                result2.WellFormed() &&
+                |result1.channels[outputIdx]| > 0 &&
+                |result2.channels[outputIdx]| > 0 &&
+                result1.channels[outputIdx][|result1.channels[outputIdx]| - 1] == result2.channels[outputIdx][|result2.channels[outputIdx]| - 1] &&
                 result1.processingElements[idx] == result2.processingElements[idx]
     {
         reveal_FirePE();
+
+        var pe := state1.processingElements[idx];
+        match pe
+            case AddOperator(a, b, outputs) => {
+                assert a in pe.WaitingInputs() && b in pe.WaitingInputs();
+                assert outputs == pe.Outputs();
+                assert a == pe.Inputs()[0] && b == pe.Inputs()[1];
+            }
+
+            case SelectOperator(d, a, b, outputs) => {
+                assert d in pe.WaitingInputs() && a in pe.WaitingInputs() && b in pe.WaitingInputs();
+                assert outputs == pe.Outputs();
+                assert d == pe.Inputs()[0] && a == pe.Inputs()[1] && b == pe.Inputs()[2];
+            }
+
+            case OrderOperator(a, b, outputs) => {
+                assert a in pe.WaitingInputs() && b in pe.WaitingInputs();
+                assert outputs <= pe.Outputs();
+                assert a == pe.Inputs()[0] && b == pe.Inputs()[1];
+            }
+
+            case _ => {}
     }
 
     lemma FirePEConfluence(idx1: PEIndex, idx2: PEIndex)
-        requires Wellformed()
+        requires WellFormed()
         requires idx1 != idx2
         requires 0 <= idx1 < |processingElements|
         requires 0 <= idx2 < |processingElements|
         requires IsFireable(idx1)
         requires IsFireable(idx2)
 
-        ensures FirePE(idx1).Wellformed()
-        ensures FirePE(idx2).Wellformed()
+        ensures FirePE(idx1).WellFormed()
+        ensures FirePE(idx2).WellFormed()
         ensures FirePE(idx1).IsFireable(idx2)
         ensures FirePE(idx2).IsFireable(idx1)
         ensures FirePE(idx1).FirePE(idx2) == FirePE(idx2).FirePE(idx1)
@@ -437,39 +530,129 @@ datatype DataflowProgramState = DataflowProgramState(channels: seq<Channel>, pro
         CommutableFiring(idx1, idx2);
         CommutableFiring(idx2, idx1);
         
+        var fired1 := FirePE(idx1);
+        var fired2 := FirePE(idx2);
         var fired12 := FirePE(idx1).FirePE(idx2);
         var fired21 := FirePE(idx2).FirePE(idx1);
 
+        var pe1 := processingElements[idx1];
+        var pe2 := processingElements[idx2];
+
+        var inputs1 := pe1.WaitingInputs();
+        var inputs2 := pe2.WaitingInputs();
+        var outputs1 := pe1.WaitingOutputs();
+        var outputs2 := pe2.WaitingOutputs();
+
         assert fired12 == fired21 by {
-            var pe1 := processingElements[idx1];
-            var pe2 := processingElements[idx2];
+            reveal_WellFormed();
+            reveal_FirePE();
 
-            var inputs1 := pe1.WaitingInputs();
-            var inputs2 := pe2.WaitingInputs();
-            var outputs1 := pe1.WaitingOutputs();
-            var outputs2 := pe2.WaitingOutputs();
+            assert fired2.processingElements[idx1] == processingElements[idx1];
+            assert fired1.processingElements[idx2] == processingElements[idx2];
+            assert |fired1.channels| == |fired2.channels| == |fired12.channels| == |fired21.channels|;
+            assert |fired1.processingElements| == |fired2.processingElements| == |fired12.processingElements| == |fired21.processingElements|;
 
-            forall i | 0 <= i < |fired12.channels|
-                ensures fired12.channels[i] == fired21.channels[i]
+            forall i | i in inputs1
+                ensures fired2.channels[i][0] == channels[i][0]
             {
-                reveal_FirePE();
-                if i in inputs1 && i in outputs1 {}
-                else if i in inputs2 && i in outputs2 {}
-                else if i in inputs1 && i in outputs2 {}
-                else if i in inputs2 && i in outputs1 {}
-                else {}
+                FirePEChannelChange(idx2, i);
             }
 
-            assert fired12.channels == fired21.channels;
+            forall i | i in inputs2
+                ensures fired1.channels[i][0] == channels[i][0]
+            {
+                FirePEChannelChange(idx1, i);
+            }
+
+            assert fired12.channels == fired21.channels by {
+                forall i | 0 <= i < |fired12.channels|
+                    ensures fired12.channels[i] == fired21.channels[i]
+                {
+                    FirePEChannelChange(idx1, i);
+                    FirePEChannelChange(idx2, i);
+                    fired2.FirePEChannelChange(idx1, i);
+                    fired1.FirePEChannelChange(idx2, i);
+
+                    if i in inputs1 && i in outputs1 {
+                        // i is a self-feeding channel
+                        FirePEDependency(this, fired2, idx1, i);
+                        assert fired21.channels[i][..|fired21.channels[i]| - 1] == fired1.channels[i][..|fired1.channels[i]| - 1];
+                        assert fired21.channels[i][|fired21.channels[i]| - 1] == fired1.channels[i][|fired1.channels[i]| - 1];
+
+                    } else if i in inputs2 && i in outputs2 {
+                        // Symmetric to the case above
+                        FirePEDependency(this, fired1, idx2, i);
+                        assert fired12.channels[i][..|fired21.channels[i]| - 1] == fired2.channels[i][..|fired2.channels[i]| - 1];
+                        assert fired12.channels[i][|fired21.channels[i]| - 1] == fired2.channels[i][|fired2.channels[i]| - 1];
+
+                    } else if i in inputs1 && i in outputs2 {
+                        // idx2 sends output via i to idx1
+                        calc {
+                            fired12.channels[i][..|fired12.channels[i]| - 1];
+                            fired1.channels[i];
+                            channels[i][1..];
+                            fired2.channels[i][1..|fired2.channels[i]| - 1];
+                            fired21.channels[i][..|fired21.channels[i]| - 1];
+                        }
+
+                        FirePEDependency(this, fired1, idx2, i);
+                        assert fired12.channels[i][|fired12.channels[i]| - 1] == fired21.channels[i][|fired21.channels[i]| - 1];
+
+                        calc {
+                            fired12.channels[i];
+                            fired12.channels[i][..|fired12.channels[i]| - 1] + [fired12.channels[i][|fired12.channels[i]| - 1]];
+                            fired21.channels[i][..|fired21.channels[i]| - 1] + [fired21.channels[i][|fired21.channels[i]| - 1]];
+                            fired21.channels[i];
+                        }
+
+                    } else if i in inputs2 && i in outputs1 {
+                        // symmetric to the case above
+                        calc {
+                            fired21.channels[i][..|fired12.channels[i]| - 1];
+                            fired1.channels[i][1..|fired1.channels[i]| - 1];
+                            channels[i][1..];
+                            fired2.channels[i];
+                            fired21.channels[i][..|fired21.channels[i]| - 1];
+                        }
+
+                        FirePEDependency(this, fired2, idx1, i);
+                        assert fired21.channels[i][|fired21.channels[i]| - 1] == fired12.channels[i][|fired12.channels[i]| - 1];
+
+                        calc {
+                            fired21.channels[i];
+                            fired21.channels[i][..|fired21.channels[i]| - 1] + [fired21.channels[i][|fired21.channels[i]| - 1]];
+                            fired12.channels[i][..|fired12.channels[i]| - 1] + [fired12.channels[i][|fired12.channels[i]| - 1]];
+                            fired12.channels[i];
+                        }
+
+                    } else if i in inputs1 && i !in outputs1 && i !in outputs2 {
+                        // i is only an input channel of idx1 but not used for anything else
+                        assert fired12.channels[i] == fired21.channels[i];
+
+                    } else if i in inputs2 && i !in outputs1 && i !in outputs2 {
+                        // i is only an input channel of idx2 but not used for anything else
+                        assert fired12.channels[i] == fired21.channels[i];
+
+                    } else if i in outputs1 && i !in inputs1 && i !in inputs2 {
+                        // i is only an output channel of idx1 but not used for anything else
+                        FirePEDependency(this, fired2, idx1, i);
+                        assert fired12.channels[i] == fired21.channels[i];
+
+                    } else if i in outputs2 && i !in inputs1 && i !in inputs2 {
+                        // i is only an output channel of idx2 but not used for anything else
+                        FirePEDependency(this, fired1, idx2, i);
+                        assert fired12.channels[i] == fired21.channels[i];
+
+                    } // else i is not changed at all
+                }
+            }
+
             assert fired12.processingElements == fired21.processingElements by {
-                reveal_FirePE();
+                assert fired1.processingElements[idx1] == fired21.processingElements[idx1];
+                assert fired2.processingElements[idx2] == fired12.processingElements[idx2];
             }
         }
-
-        // assert FirePE(idx1).Wellformed();
-        // assert FirePE(idx2).Wellformed();
-        // assert FirePE(idx1).IsFireable(idx2);
-        // assert FirePE(idx2).IsFireable(idx1);
-        // assert FirePE(idx1).FirePE(idx2) == FirePE(idx2).FirePE(idx1);
+        
+        assert FirePE(idx1).FirePE(idx2) == FirePE(idx2).FirePE(idx1);
     }
 }
